feat: add SEnv

CollapsingTowers/TwoLevelPCP/Typing.lean
@@ -3,6 +3,7 @@ import CollapsingTowers.TwoLevelPCP.Syntax
 import CollapsingTowers.TwoLevelPCP.Shift
 import CollapsingTowers.TwoLevelPCP.SmallStep
 import CollapsingTowers.TwoLevelPCP.Env
+import CollapsingTowers.TwoLevelPCP.Store
 @[simp]
 def well_binding_time : Stage → Ty → Prop
   | .stat, .nat => true
@@ -29,178 +30,187 @@ theorem well_binding_time_escape : ∀ 𝕊 τ, well_binding_time 𝕊 τ → we
     | rep => nomatch HwellBinds
 
 mutual
-  inductive typing : TEnv → Stage → Expr → Ty → Effects → Prop where
-    | fvar : ∀ Γ 𝕊 x τ,
+  inductive typing : TEnv → SEnv → Stage → Expr → Ty → Effects → Prop where
+    | fvar : ∀ Γ σ 𝕊 x τ,
       binds x (τ, 𝕊) Γ →
       well_binding_time 𝕊 τ →
-      typing Γ 𝕊 (.fvar x) τ ∅
-    | lam₁ : ∀ Γ 𝕊 e τ𝕒 τ𝕓 φ,
-      typing ((τ𝕒, 𝕊) :: Γ) 𝕊 (open₀ Γ.length e) τ𝕓 φ →
+      typing Γ σ 𝕊 (.fvar x) τ ∅
+    | lam₁ : ∀ Γ σ 𝕊 e τ𝕒 τ𝕓 φ,
+      typing ((τ𝕒, 𝕊) :: Γ) σ 𝕊 (open₀ Γ.length e) τ𝕓 φ →
       well_binding_time 𝕊 τ𝕒 →
       closed_at e Γ.length →
-      typing Γ 𝕊 (.lam₁ e) (.arrow τ𝕒 τ𝕓 φ) ∅
-    | lift_lam : ∀ Γ e τ𝕒 τ𝕓 φ₀ φ₁,
-      typing Γ .stat e (.arrow (.fragment τ𝕒) (.fragment τ𝕓) φ₀) φ₁ →
-      typing Γ .stat (.lift e) (.fragment (.arrow τ𝕒 τ𝕓 ∅)) .reify
-    | app₁ : ∀ Γ 𝕊 f arg τ𝕒 τ𝕓 φ₀ φ₁ φ₂,
-      typing Γ 𝕊 f (.arrow τ𝕒 τ𝕓 φ₀) φ₁ →
-      typing Γ 𝕊 arg τ𝕒 φ₂ →
-      typing Γ 𝕊 (.app₁ f arg) τ𝕓 (φ₀ ∪ φ₁ ∪ φ₂)
-    | app₂ : ∀ Γ f arg τ𝕒 τ𝕓 φ₀ φ₁,
-      typing Γ .stat f (.fragment (.arrow τ𝕒 τ𝕓 ∅)) φ₀ →
-      typing Γ .stat arg (.fragment τ𝕒) φ₁ →
-      typing Γ .stat (.app₂ f arg) (.fragment τ𝕓) .reify
-    | plus₁ : ∀ Γ 𝕊 l r φ₀ φ₁,
-      typing Γ 𝕊 l .nat φ₀ →
-      typing Γ 𝕊 r .nat φ₁ →
-      typing Γ 𝕊 (.plus₁ l r) .nat (φ₀ ∪ φ₁)
-    | plus₂ : ∀ Γ l r φ₀ φ₁,
-      typing Γ .stat l (.fragment .nat) φ₀ →
-      typing Γ .stat r (.fragment .nat) φ₁ →
-      typing Γ .stat (.plus₂ l r) (.fragment .nat) .reify
-    | lit₁ : ∀ Γ 𝕊 n,
-      typing Γ 𝕊 (.lit₁ n) .nat ∅
-    | lift_lit : ∀ Γ n φ,
-      typing Γ .stat n .nat φ →
-      typing Γ .stat (.lift n) (.fragment .nat) .reify
-    | code_fragment : ∀ Γ x τ,
+      typing Γ σ 𝕊 (.lam₁ e) (.arrow τ𝕒 τ𝕓 φ) ∅
+    | lift_lam : ∀ Γ σ e τ𝕒 τ𝕓 φ₀ φ₁,
+      typing Γ σ .stat e (.arrow (.fragment τ𝕒) (.fragment τ𝕓) φ₀) φ₁ →
+      typing Γ σ .stat (.lift e) (.fragment (.arrow τ𝕒 τ𝕓 ∅)) .reify
+    | app₁ : ∀ Γ σ 𝕊 f arg τ𝕒 τ𝕓 φ₀ φ₁ φ₂,
+      typing Γ σ 𝕊 f (.arrow τ𝕒 τ𝕓 φ₀) φ₁ →
+      typing Γ σ 𝕊 arg τ𝕒 φ₂ →
+      typing Γ σ 𝕊 (.app₁ f arg) τ𝕓 (φ₀ ∪ φ₁ ∪ φ₂)
+    | app₂ : ∀ Γ σ f arg τ𝕒 τ𝕓 φ₀ φ₁,
+      typing Γ σ .stat f (.fragment (.arrow τ𝕒 τ𝕓 ∅)) φ₀ →
+      typing Γ σ .stat arg (.fragment τ𝕒) φ₁ →
+      typing Γ σ .stat (.app₂ f arg) (.fragment τ𝕓) .reify
+    | plus₁ : ∀ Γ σ 𝕊 l r φ₀ φ₁,
+      typing Γ σ 𝕊 l .nat φ₀ →
+      typing Γ σ 𝕊 r .nat φ₁ →
+      typing Γ σ 𝕊 (.plus₁ l r) .nat (φ₀ ∪ φ₁)
+    | plus₂ : ∀ Γ σ l r φ₀ φ₁,
+      typing Γ σ .stat l (.fragment .nat) φ₀ →
+      typing Γ σ .stat r (.fragment .nat) φ₁ →
+      typing Γ σ .stat (.plus₂ l r) (.fragment .nat) .reify
+    | lit₁ : ∀ Γ σ 𝕊 n,
+      typing Γ σ 𝕊 (.lit₁ n) .nat ∅
+    | lift_lit : ∀ Γ σ n φ,
+      typing Γ σ .stat n .nat φ →
+      typing Γ σ .stat (.lift n) (.fragment .nat) .reify
+    | code_fragment : ∀ Γ σ x τ,
       binds x (τ, .dyn) Γ →
       well_binding_time .dyn τ →
-      typing Γ .stat (.code (.fvar x)) (.fragment τ) ∅
-    | code_rep : ∀ Γ e τ,
-      typing Γ .dyn e τ ∅ →
-      typing Γ .stat (.code e) (.rep τ) ∅
-    | reflect : ∀ Γ e τ,
-      typing Γ .dyn e τ ∅ →
-      typing Γ .stat (.reflect e) (.fragment τ) .reify
-    | lam𝕔 : ∀ Γ e τ𝕒 τ𝕓 φ,
-      typing_reification ((τ𝕒, .dyn) :: Γ) (open₀ Γ.length e) (.rep τ𝕓) φ →
+      typing Γ σ .stat (.code (.fvar x)) (.fragment τ) ∅
+    | code_rep : ∀ Γ σ e τ,
+      typing Γ σ .dyn e τ ∅ →
+      typing Γ σ .stat (.code e) (.rep τ) ∅
+    | reflect : ∀ Γ σ e τ,
+      typing Γ σ .dyn e τ ∅ →
+      typing Γ σ .stat (.reflect e) (.fragment τ) .reify
+    | lam𝕔 : ∀ Γ σ e τ𝕒 τ𝕓 φ,
+      typing_reification ((τ𝕒, .dyn) :: Γ) σ (open₀ Γ.length e) (.rep τ𝕓) φ →
       well_binding_time .dyn τ𝕒 →
       closed_at e Γ.length →
-      typing Γ .stat (.lam𝕔 e) (.fragment (.arrow τ𝕒 τ𝕓 ∅)) .reify
-    | lets : ∀ Γ 𝕊 b e τ𝕒 τ𝕓 φ₀ φ₁,
-      typing Γ 𝕊 b τ𝕒 φ₀ →
-      typing ((τ𝕒, 𝕊) :: Γ) 𝕊 (open₀ Γ.length e) τ𝕓 φ₁ →
+      typing Γ σ .stat (.lam𝕔 e) (.fragment (.arrow τ𝕒 τ𝕓 ∅)) .reify
+    | lets : ∀ Γ σ 𝕊 b e τ𝕒 τ𝕓 φ₀ φ₁,
+      typing Γ σ 𝕊 b τ𝕒 φ₀ →
+      typing ((τ𝕒, 𝕊) :: Γ) σ 𝕊 (open₀ Γ.length e) τ𝕓 φ₁ →
       well_binding_time 𝕊 τ𝕒 →
       closed_at e Γ.length →
-      typing Γ 𝕊 (.lets b e) τ𝕓 (φ₀ ∪ φ₁)
-    | let𝕔 : ∀ Γ b e τ𝕒 τ𝕓 φ,
-      typing Γ .dyn b τ𝕒 ∅ →
-      typing_reification ((τ𝕒, .dyn) :: Γ) (open₀ Γ.length e) (.rep τ𝕓) φ →
+      typing Γ σ 𝕊 (.lets b e) τ𝕓 (φ₀ ∪ φ₁)
+    | let𝕔 : ∀ Γ σ b e τ𝕒 τ𝕓 φ,
+      typing Γ σ .dyn b τ𝕒 ∅ →
+      typing_reification ((τ𝕒, .dyn) :: Γ) σ (open₀ Γ.length e) (.rep τ𝕓) φ →
       well_binding_time .dyn τ𝕒 →
       closed_at e Γ.length →
-      typing Γ .stat (.let𝕔 b e) (.rep τ𝕓) ∅
-    | run : ∀ Γ e τ φ,
-      typing_reification Γ e (.rep τ) φ →
+      typing Γ σ .stat (.let𝕔 b e) (.rep τ𝕓) ∅
+    | run : ∀ Γ σ e τ φ,
+      typing_reification Γ σ e (.rep τ) φ →
       closed_at e 0 →
-      typing Γ .stat (.run e) τ ∅
+      typing Γ σ .stat (.run e) τ ∅
 
-  inductive typing_reification : TEnv → Expr → Ty → Effects → Prop
-    | pure : ∀ Γ e τ, typing Γ .stat e τ ∅ → typing_reification Γ e τ ∅
-    | reify : ∀ Γ e τ φ, typing Γ .stat e (.fragment τ) φ → typing_reification Γ e (.rep τ) φ
+  inductive typing_reification : TEnv → SEnv → Expr → Ty → Effects → Prop
+    | pure : ∀ Γ σ e τ, typing Γ σ .stat e τ ∅ → typing_reification Γ σ e τ ∅
+    | reify : ∀ Γ σ e τ φ, typing Γ σ .stat e (.fragment τ) φ → typing_reification Γ σ e (.rep τ) φ
 end
 
-theorem typing_regular : ∀ Γ 𝕊 e τ φ, typing Γ 𝕊 e τ φ → lc e :=
+@[simp]
+def well_store (st : Store) (σ : SEnv) : Prop :=
+  σ.length = st.length ∧
+  (∀ loc e,
+    binds loc e st →
+    binds loc .nat σ →
+    typing [] σ .stat e .nat ∅
+  )
+
+theorem typing_regular : ∀ Γ σ 𝕊 e τ φ, typing Γ σ 𝕊 e τ φ → lc e :=
   by
-  intros Γ 𝕊 e τ φ Hτ
+  intros Γ σ 𝕊 e τ φ Hτ
   apply
     @typing.rec
-      (fun Γ 𝕊 e τ φ (H : typing Γ 𝕊 e τ φ) => lc e)
-      (fun Γ e τ φ (H : typing_reification Γ e τ φ) => lc e)
+      (fun Γ σ 𝕊 e τ φ (H : typing Γ σ 𝕊 e τ φ) => lc e)
+      (fun Γ σ e τ φ (H : typing_reification Γ σ e τ φ) => lc e)
   <;> (try simp)
   case lam₁ =>
-    intros _ _ _ _ _ _ _ _ _ IH
+    intros _ _ _ _ _ _ _ _ _ _ IH
     apply open_closedb; apply IH
   case lam𝕔 =>
-    intros _ _ _ _ _ _ _ _ IH
+    intros _ _ _ _ _ _ _ _ _ IH
     apply open_closedb; apply IH
   case app₁ =>
-    intros _ _ _ _ _ _ _ _ _ _ _ IHf IHarg
+    intros _ _ _ _ _ _ _ _ _ _ _ _ IHf IHarg
     constructor; apply IHf; apply IHarg
   case app₂ =>
-    intros _ _ _ _ _ _ _ _ _ IHf IHarg
+    intros _ _ _ _ _ _ _ _ _ _ IHf IHarg
     constructor; apply IHf; apply IHarg
   case plus₁ =>
-    intros _ _ _ _ _ _ _ _ IHl IHr
+    intros _ _ _ _ _ _ _ _ _ IHl IHr
     constructor; apply IHl; apply IHr
   case plus₂ =>
-    intros _ _ _ _ _ _ _ IHl IHr
+    intros _ _ _ _ _ _ _ _ IHl IHr
     constructor; apply IHl; apply IHr
   case lets =>
-    intros _ _ _ _ _ _ _ _ _ _ _ _ IHb IHe
+    intros _ _ _ _ _ _ _ _ _ _ _ _ _ IHb IHe
     constructor
     apply IHb; apply open_closedb; apply IHe
   case let𝕔 =>
-    intros _ _ _ _ _ _ _ _ _ _ IHb IHe
+    intros _ _ _ _ _ _ _ _ _ _ _ IHb IHe
     constructor
     apply IHb; apply open_closedb; apply IHe
   apply Hτ
 
-theorem typing_closed : ∀ Γ 𝕊 e τ φ, typing Γ 𝕊 e τ φ → closed_at e Γ.length :=
+theorem typing_closed : ∀ Γ σ 𝕊 e τ φ, typing Γ σ 𝕊 e τ φ → closed_at e Γ.length :=
   by
-  intros Γ 𝕊 e τ φ Hτ
+  intros Γ σ 𝕊 e τ φ Hτ
   apply
     @typing.rec
-      (fun Γ 𝕊 e τ φ (H : typing Γ 𝕊 e τ φ) => closed_at e Γ.length)
-      (fun Γ e τ φ (H : typing_reification Γ e τ φ) => closed_at e Γ.length)
+      (fun Γ σ 𝕊 e τ φ (H : typing Γ σ 𝕊 e τ φ) => closed_at e Γ.length)
+      (fun Γ σ e τ φ (H : typing_reification Γ σ e τ φ) => closed_at e Γ.length)
   <;> (try intros; assumption)
   case fvar =>
-    intros _ _ _ _ Hbinds _
+    intros _ _ _ _ _ Hbinds _
     apply indexr_iff_lt.mpr; constructor
     apply Hbinds
   case app₁ =>
-    intros _ _ _ _ _ _ _ _ _ _ _ IHf IHarg
+    intros _ _ _ _ _ _ _ _ _ _ _ _ IHf IHarg
     constructor; apply IHf; apply IHarg
   case app₂ =>
-    intros _ _ _ _ _ _ _ _ _ IHf IHarg
+    intros _ _ _ _ _ _ _ _ _ _ IHf IHarg
     constructor; apply IHf; apply IHarg
   case plus₁ =>
-    intros _ _ _ _ _ _ _ _ IHl IHr
+    intros _ _ _ _ _ _ _ _ _ IHl IHr
     constructor; apply IHl; apply IHr
   case plus₂ =>
-    intros _ _ _ _ _ _ _ IHl IHr
+    intros _ _ _ _ _ _ _ _ IHl IHr
     constructor; apply IHl; apply IHr
   case lit₁ => simp
   case code_fragment =>
-    intros _ _ _ Hbinds _
+    intros _ _ _ _ Hbinds _
     apply indexr_iff_lt.mpr; constructor
     apply Hbinds
   case lets =>
-    intros _ _ _ _ _ _ _ _ _ _ _ Hclose IHb _
+    intros _ _ _ _ _ _ _ _ _ _ _ _ Hclose IHb _
     constructor; apply IHb; apply Hclose
   case let𝕔 =>
-    intros _ _ _ _ _ _ _ _ _ Hclose IHb _
+    intros _ _ _ _ _ _ _ _ _ _ Hclose IHb _
     constructor; apply IHb; apply Hclose
 
-theorem typing_reification_closed : ∀ Γ e τ φ, typing_reification Γ e τ φ → closed_at e Γ.length :=
+theorem typing_reification_closed : ∀ Γ σ e τ φ, typing_reification Γ σ e τ φ → closed_at e Γ.length :=
   by
-  intros Γ e τ φ Hτ
+  intros Γ σ e τ φ Hτ
   cases Hτ
   all_goals
     next Hτ =>
       apply typing_closed
       apply Hτ
 
-theorem typing_value_pure : ∀ Γ v τ φ, typing Γ .stat v τ φ → value v → φ = ∅ :=
+theorem typing_value_pure : ∀ Γ σ v τ φ, typing Γ σ .stat v τ φ → value v → φ = ∅ :=
   by
-  intros _ _ _ _ Hτ Hvalue
+  intros _ _ _ _ _ Hτ Hvalue
   cases Hvalue <;> cases Hτ <;> rfl
 
-theorem typing_dyn_pure : ∀ Γ e τ φ, typing Γ .dyn e τ φ → well_binding_time .dyn τ ∧ φ = ∅ :=
+theorem typing_dyn_pure : ∀ Γ σ e τ φ, typing Γ σ .dyn e τ φ → well_binding_time .dyn τ ∧ φ = ∅ :=
   by
   generalize HEq𝕊 : (.dyn : Stage) = 𝕊
-  intros Γ e τ φ Hτ
+  intros Γ σ e τ φ Hτ
   revert HEq𝕊
   apply @typing.rec
-    (fun Γ 𝕊 e τ φ (H : typing Γ 𝕊 e τ φ) => .dyn = 𝕊 → well_binding_time 𝕊 τ ∧ φ = ∅)
-    (fun Γ e τ φ (H : typing_reification Γ e τ φ) => true)
+    (fun Γ σ 𝕊 e τ φ (H : typing Γ σ 𝕊 e τ φ) => .dyn = 𝕊 → well_binding_time 𝕊 τ ∧ φ = ∅)
+    (fun Γ σ e τ φ (H : typing_reification Γ σ e τ φ) => true)
   <;> (try intros; assumption)
   <;> (try intros; contradiction)
   case fvar =>
-    intros _ _ x _ Hbinds HwellBinds HEq𝕊
+    intros _ _ _ x _ Hbinds HwellBinds HEq𝕊
     constructor; apply HwellBinds; rfl
   case lam₁ =>
-    intros _ _ _ _ _ _ _ HwellBinds₀ Hclose IH HEq𝕊
+    intros _ _ _ _ _ _ _ _ HwellBinds₀ Hclose IH HEq𝕊
     have ⟨HwellBinds₁, Hφ₀⟩ := IH HEq𝕊
     rw [← HEq𝕊]
     rw [← HEq𝕊] at HwellBinds₀ HwellBinds₁
@@ -210,7 +220,7 @@ theorem typing_dyn_pure : ∀ Γ e τ φ, typing Γ .dyn e τ φ → well_bindin
       apply HwellBinds₀; apply HwellBinds₁
     . rfl
   case app₁ =>
-    intros _ _ _ _ _ _ _ _ _ _ _ IHf IHarg HEq𝕊
+    intros _ _ _ _ _ _ _ _ _ _ _ _ IHf IHarg HEq𝕊
     have ⟨HwellBinds₁, Hφ₁⟩ := IHf HEq𝕊
     have ⟨HwellBinds₂, Hφ₂⟩ := IHarg HEq𝕊
     rw [← HEq𝕊]
@@ -219,7 +229,7 @@ theorem typing_dyn_pure : ∀ Γ e τ φ, typing Γ .dyn e τ φ → well_bindin
     . apply HwellBinds₁.right.right
     . rw [Hφ₁, Hφ₂, HwellBinds₁.left]; rfl
   case plus₁ =>
-    intros _ _ _ _ _ _ _ _ IHl IHr HEq𝕊
+    intros _ _ _ _ _ _ _ _ _ IHl IHr HEq𝕊
     have ⟨HwellBinds₁, Hφ₁⟩ := IHl HEq𝕊
     have ⟨HwellBinds₂, Hφ₂⟩ := IHr HEq𝕊
     rw [← HEq𝕊]
@@ -227,13 +237,13 @@ theorem typing_dyn_pure : ∀ Γ e τ φ, typing Γ .dyn e τ φ → well_bindin
     . simp
     . rw [Hφ₁, Hφ₂]; rfl
   case lit₁ =>
-    intros _ _ _ HEq𝕊
+    intros _ _ _ _ HEq𝕊
     rw [← HEq𝕊]
     constructor
     . simp
     . rfl
   case lets =>
-    intros _ _ _ _ _ _ _ _ _ _ HwellBinds Hclose IHb IHe HEq𝕊
+    intros _ _ _ _ _ _ _ _ _ _ _ HwellBinds Hclose IHb IHe HEq𝕊
     have ⟨HwellBinds₁, Hφ₁⟩ := IHb HEq𝕊
     have ⟨HwellBinds₂, Hφ₂⟩ := IHe HEq𝕊
     constructor
@@ -243,28 +253,28 @@ theorem typing_dyn_pure : ∀ Γ e τ φ, typing Γ .dyn e τ φ → well_bindin
   case reify => simp
 
 theorem typing_shrink_strengthened :
-  ∀ Γ Ψ Δ Φ 𝕊 e τ φ,
-    typing Γ 𝕊 e τ φ →
+  ∀ Γ Ψ Δ Φ σ 𝕊 e τ φ,
+    typing Γ σ 𝕊 e τ φ →
     Γ = Ψ ++ Φ :: Δ →
     Δ.length ∉ fv e →
-    typing (Ψ ++ Δ) 𝕊 (shiftr_at Δ.length e) τ φ :=
+    typing (Ψ ++ Δ) σ 𝕊 (shiftr_at Δ.length e) τ φ :=
   by
-  intros Γ Ψ Δ Φ 𝕊 e τ φ Hτ
+  intros Γ Ψ Δ Φ σ 𝕊 e τ φ Hτ
   revert Ψ
   apply
     @typing.rec
-      (fun Γ 𝕊 e τ φ (H : typing Γ 𝕊 e τ φ) =>
+      (fun Γ σ 𝕊 e τ φ (H : typing Γ σ 𝕊 e τ φ) =>
         ∀ Ψ,
           Γ = Ψ ++ Φ :: Δ →
           Δ.length ∉ fv e →
-          typing (Ψ ++ Δ) 𝕊 (shiftr_at Δ.length e) τ φ)
-      (fun Γ e τ φ (H : typing_reification Γ e τ φ) =>
+          typing (Ψ ++ Δ) σ 𝕊 (shiftr_at Δ.length e) τ φ)
+      (fun Γ σ e τ φ (H : typing_reification Γ σ e τ φ) =>
         ∀ Ψ,
           Γ = Ψ ++ Φ :: Δ →
           Δ.length ∉ fv e →
-          typing_reification (Ψ ++ Δ) (shiftr_at Δ.length e) τ φ)
+          typing_reification (Ψ ++ Δ) σ (shiftr_at Δ.length e) τ φ)
   case fvar =>
-    intros _ _ x _ Hbinds HwellBinds Ψ HEqΓ HcloseΔ
+    intros _ _ _ x _ Hbinds HwellBinds Ψ HEqΓ HcloseΔ
     rw [HEqΓ] at Hbinds; simp
     cases Hx : compare Δ.length x with
     | lt =>
@@ -288,7 +298,7 @@ theorem typing_shrink_strengthened :
       apply binds_extend; apply binds_shrink
       omega; rw [List.append_cons] at Hbinds; apply Hbinds; apply HwellBinds
   case lam₁ =>
-    intros _ _ _ _ _ _ _ HwellBinds Hclose IH Ψ HEqΓ HcloseΔ
+    intros _ _ _ _ _ _ _ _ HwellBinds Hclose IH Ψ HEqΓ HcloseΔ
     rw [HEqΓ, shiftr_open₀_comm] at IH
     rw [HEqΓ] at Hclose
     apply typing.lam₁
@@ -307,11 +317,11 @@ theorem typing_shrink_strengthened :
       apply Hclose
     simp; omega
   case lift_lam =>
-    intros _ _ _ _ _ _ _ IH Ψ HEqΓ HcloseΔ
+    intros _ _ _ _ _ _ _ _ IH Ψ HEqΓ HcloseΔ
     apply typing.lift_lam
     apply IH; apply HEqΓ; apply HcloseΔ
   case lam𝕔 =>
-    intros _ _ _ _ _ _ HwellBinds Hclose IH Ψ HEqΓ HcloseΔ
+    intros _ _ _ _ _ _ _ HwellBinds Hclose IH Ψ HEqΓ HcloseΔ
     rw [HEqΓ] at IH; rw [HEqΓ] at Hclose
     rw [shiftr_open₀_comm] at IH
     apply typing.lam𝕔
@@ -330,32 +340,32 @@ theorem typing_shrink_strengthened :
       apply Hclose
     simp; omega
   case app₁ =>
-    intros _ _ _ _ _ _ _ _ _ _ _ IHf IHarg Ψ HEqΓ HcloseΔ
+    intros _ _ _ _ _ _ _ _ _ _ _ _ IHf IHarg Ψ HEqΓ HcloseΔ
     simp at HcloseΔ; apply typing.app₁
     apply IHf; apply HEqΓ; apply HcloseΔ.left
     apply IHarg; apply HEqΓ; apply HcloseΔ.right
   case app₂ =>
-    intros _ _ _ _ _ _ _ _ _ IHf IHarg Ψ HEqΓ HcloseΔ
+    intros _ _ _ _ _ _ _ _ _ _ IHf IHarg Ψ HEqΓ HcloseΔ
     simp at HcloseΔ; apply typing.app₂
     apply IHf; apply HEqΓ; apply HcloseΔ.left
     apply IHarg; apply HEqΓ; apply HcloseΔ.right
   case plus₁ =>
-    intros _ _ _ _ _ _ _ _ IHl IHr Ψ HEqΓ HcloseΔ
+    intros _ _ _ _ _ _ _ _ _ IHl IHr Ψ HEqΓ HcloseΔ
     simp at HcloseΔ; apply typing.plus₁
     apply IHl; apply HEqΓ; apply HcloseΔ.left
     apply IHr; apply HEqΓ; apply HcloseΔ.right
   case plus₂ =>
-    intros _ _ _ _ _ _ _ IHl IHr Ψ HEqΓ HcloseΔ
+    intros _ _ _ _ _ _ _ _ IHl IHr Ψ HEqΓ HcloseΔ
     simp at HcloseΔ; apply typing.plus₂
     apply IHl; apply HEqΓ; apply HcloseΔ.left
     apply IHr; apply HEqΓ; apply HcloseΔ.right
   case lit₁ => intros; apply typing.lit₁
   case lift_lit =>
-    intros _ _ _ _ IH Ψ HEqΓ HcloseΔ
+    intros _ _ _ _ _ IH Ψ HEqΓ HcloseΔ
     apply typing.lift_lit
     apply IH; apply HEqΓ; apply HcloseΔ
   case code_fragment =>
-    intros _ x _ Hbinds HwellBinds Ψ HEqΓ HcloseΔ
+    intros _ _ x _ Hbinds HwellBinds Ψ HEqΓ HcloseΔ
     rw [HEqΓ] at Hbinds; simp
     cases Hx : compare Δ.length x with
     | lt =>
@@ -379,15 +389,15 @@ theorem typing_shrink_strengthened :
       apply binds_extend; apply binds_shrink
       omega; rw [List.append_cons] at Hbinds; apply Hbinds; apply HwellBinds
   case code_rep =>
-    intros _ _ _ _ IH Ψ HEqΓ HcloseΔ
+    intros _ _ _ _ _ IH Ψ HEqΓ HcloseΔ
     apply typing.code_rep
     apply IH; apply HEqΓ; apply HcloseΔ
   case reflect =>
-    intros _ _ _ _ IH Ψ HEqΓ HcloseΔ
+    intros _ _ _ _ _ IH Ψ HEqΓ HcloseΔ
     apply typing.reflect
     apply IH; apply HEqΓ; apply HcloseΔ
   case lets =>
-    intros _ _ _ _ _ _ _ _ _ _ HwellBinds Hclose IHb IHe Ψ HEqΓ HcloseΔ
+    intros _ _ _ _ _ _ _ _ _ _ _ HwellBinds Hclose IHb IHe Ψ HEqΓ HcloseΔ
     rw [HEqΓ] at IHb; rw [HEqΓ] at IHe; rw [HEqΓ] at Hclose
     rw [shiftr_open₀_comm] at IHe
     simp at IHb; simp at IHe; simp at HcloseΔ
@@ -407,7 +417,7 @@ theorem typing_shrink_strengthened :
       apply Hclose
     simp; omega
   case let𝕔 =>
-    intros _ _ _ _ _ _ _ _ HwellBinds Hclose IHb IHe Ψ HEqΓ HcloseΔ
+    intros _ _ _ _ _ _ _ _ _ HwellBinds Hclose IHb IHe Ψ HEqΓ HcloseΔ
     rw [HEqΓ] at IHb; rw [HEqΓ] at IHe; rw [HEqΓ] at Hclose
     rw [shiftr_open₀_comm] at IHe
     simp at IHb; simp at IHe; simp at HcloseΔ
@@ -427,51 +437,51 @@ theorem typing_shrink_strengthened :
       apply Hclose
     simp; omega
   case run =>
-    intros _ _ _ _ _ Hclose IH Ψ HEqΓ HcloseΔ
+    intros _ _ _ _ _ _ Hclose IH Ψ HEqΓ HcloseΔ
     apply typing.run
     apply IH; apply HEqΓ; apply HcloseΔ
     rw [shiftr_id]; apply Hclose
     apply closed_inc; apply Hclose; omega
   case pure =>
-    intros _ _ _ _ IH Ψ HEqΓ HcloseΔ
+    intros _ _ _ _ _ IH Ψ HEqΓ HcloseΔ
     apply typing_reification.pure
     apply IH; apply HEqΓ; apply HcloseΔ
   case reify =>
-    intros _ _ _ _ _ IH Ψ HEqΓ HcloseΔ
+    intros _ _ _ _ _ _ IH Ψ HEqΓ HcloseΔ
     apply typing_reification.reify
     apply IH; apply HEqΓ; apply HcloseΔ
   apply Hτ
 
 theorem typing_shrink :
-  ∀ Γ Φ 𝕊 e τ φ,
-    typing (Φ :: Γ) 𝕊 e τ φ →
+  ∀ Γ Φ σ 𝕊 e τ φ,
+    typing (Φ :: Γ) σ 𝕊 e τ φ →
     closed_at e Γ.length →
-    typing Γ 𝕊 e τ φ :=
+    typing Γ σ 𝕊 e τ φ :=
   by
-  intros Γ Φ 𝕊 e τ φ Hτ Hclose
-  have H := typing_shrink_strengthened (Φ :: Γ) [] Γ Φ 𝕊 e τ φ
+  intros Γ Φ σ 𝕊 e τ φ Hτ Hclose
+  have H := typing_shrink_strengthened (Φ :: Γ) [] Γ Φ σ 𝕊 e τ φ
   rw [shiftr_id] at H
   apply H; apply Hτ; rfl
   apply fv_if_closed_at; apply Hclose; omega
   apply closed_inc; apply Hclose; omega
 
 theorem weakening_strengthened :
-    ∀ Γ Ψ Δ Φ 𝕊 e τ φ, typing Γ 𝕊 e τ φ → Γ = Ψ ++ Φ → typing (Ψ ++ Δ ++ Φ) 𝕊 (shiftl_at Φ.length Δ.length e) τ φ :=
+    ∀ Γ Ψ Δ Φ σ 𝕊 e τ φ, typing Γ σ 𝕊 e τ φ → Γ = Ψ ++ Φ → typing (Ψ ++ Δ ++ Φ) σ 𝕊 (shiftl_at Φ.length Δ.length e) τ φ :=
   by
-  intros Γ Ψ Δ Φ 𝕊 e τ φ Hτ HEqΓ
+  intros Γ Ψ Δ Φ σ 𝕊 e τ φ Hτ HEqΓ
   revert Ψ
   apply
     @typing.rec
-      (fun Γ 𝕊 e τ φ (H : typing Γ 𝕊 e τ φ) =>
+      (fun Γ σ 𝕊 e τ φ (H : typing Γ σ 𝕊 e τ φ) =>
         ∀ Ψ,
           Γ = Ψ ++ Φ →
-          typing (Ψ ++ Δ ++ Φ) 𝕊 (shiftl_at (List.length Φ) (List.length Δ) e) τ φ)
-      (fun Γ e τ φ (H : typing_reification Γ e τ φ) =>
+          typing (Ψ ++ Δ ++ Φ) σ 𝕊 (shiftl_at (List.length Φ) (List.length Δ) e) τ φ)
+      (fun Γ σ e τ φ (H : typing_reification Γ σ e τ φ) =>
         ∀ Ψ,
           Γ = Ψ ++ Φ →
-          typing_reification (Ψ ++ Δ ++ Φ) (shiftl_at (List.length Φ) (List.length Δ) e) τ φ)
+          typing_reification (Ψ ++ Δ ++ Φ) σ (shiftl_at (List.length Φ) (List.length Δ) e) τ φ)
   case fvar =>
-    intros _ _ x _ Hbinds HwellBinds Ψ HEqΓ
+    intros _ _ _ x _ Hbinds HwellBinds Ψ HEqΓ
     rw [HEqΓ] at Hbinds
     by_cases HLe : Φ.length <= x
     . simp only [shiftl_at]; rw [if_pos HLe]; apply typing.fvar
@@ -485,7 +495,7 @@ theorem weakening_strengthened :
       apply binds_extend; apply binds_shrink
       omega; apply Hbinds; apply HwellBinds
   case lam₁ =>
-    intros _ _ _ _ _ _ _ HwellBinds Hclose IH Ψ HEqΓ
+    intros _ _ _ _ _ _ _ _ HwellBinds Hclose IH Ψ HEqΓ
     rw [HEqΓ] at IH
     rw [HEqΓ] at Hclose
     rw [shiftl_open₀_comm] at IH
@@ -496,11 +506,11 @@ theorem weakening_strengthened :
     rw [List.length_append, List.length_append, Nat.add_right_comm]
     apply shiftl_closed_at; rw [← List.length_append]; apply Hclose; simp
   case lift_lam =>
-    intros _ _ _ _ _ _ _ IH Ψ HEqΓ
+    intros _ _ _ _ _ _ _ _ IH Ψ HEqΓ
     apply typing.lift_lam
     apply IH; apply HEqΓ
   case lam𝕔 =>
-    intros _ _ _ _ _ _ HwellBinds Hclose IH Ψ HEqΓ
+    intros _ _ _ _ _ _ _ HwellBinds Hclose IH Ψ HEqΓ
     rw [HEqΓ] at IH
     rw [HEqΓ] at Hclose
     rw [shiftl_open₀_comm] at IH
@@ -511,32 +521,32 @@ theorem weakening_strengthened :
     rw [List.length_append, List.length_append, Nat.add_right_comm]
     apply shiftl_closed_at; rw [← List.length_append]; apply Hclose; simp
   case app₁ =>
-    intros _ _ _ _ _ _ _ _ _ _ _ IHf IHarg Ψ HEqΓ
+    intros _ _ _ _ _ _ _ _ _ _ _ _ IHf IHarg Ψ HEqΓ
     apply typing.app₁
     apply IHf; apply HEqΓ
     apply IHarg; apply HEqΓ
   case app₂ =>
-    intros _ _ _ _ _ _ _ _ _ IHf IHarg Ψ HEqΓ
+    intros _ _ _ _ _ _ _ _ _ _ IHf IHarg Ψ HEqΓ
     apply typing.app₂
     apply IHf; apply HEqΓ
     apply IHarg; apply HEqΓ
   case plus₁ =>
-    intros _ _ _ _ _ _ _ _ IHl IHr Ψ HEqΓ
+    intros _ _ _ _ _ _ _ _ _ IHl IHr Ψ HEqΓ
     apply typing.plus₁
     apply IHl; apply HEqΓ
     apply IHr; apply HEqΓ
   case plus₂ =>
-    intros _ _ _ _ _ _ _ IHl IHr Ψ HEqΓ
+    intros _ _ _ _ _ _ _ _ IHl IHr Ψ HEqΓ
     apply typing.plus₂
     apply IHl; apply HEqΓ
     apply IHr; apply HEqΓ
   case lit₁ => intros; apply typing.lit₁
   case lift_lit =>
-    intros _ _ _ _ IH Ψ HEqΓ
+    intros _ _ _ _ _ IH Ψ HEqΓ
     apply typing.lift_lit
     apply IH; apply HEqΓ
   case code_fragment =>
-    intros _ x _ Hbinds HwellBinds Ψ HEqΓ
+    intros _ _ x _ Hbinds HwellBinds Ψ HEqΓ
     rw [HEqΓ] at Hbinds
     by_cases HLe : Φ.length <= x
     . simp only [shiftl_at]; rw [if_pos HLe]; apply typing.code_fragment
@@ -550,15 +560,15 @@ theorem weakening_strengthened :
       apply binds_extend; apply binds_shrink
       omega; apply Hbinds; apply HwellBinds
   case code_rep =>
-    intros _ _ _ _ IH Ψ HEqΓ
+    intros _ _ _ _ _ IH Ψ HEqΓ
     apply typing.code_rep
     apply IH; apply HEqΓ
   case reflect =>
-    intros _ _ _ _ IH Ψ HEqΓ
+    intros _ _ _ _ _ IH Ψ HEqΓ
     apply typing.reflect
     apply IH; apply HEqΓ
   case lets =>
-    intros _ _ _ _ _ _ _ _ _ _ HwellBinds Hclose IHb IHe Ψ HEqΓ
+    intros _ _ _ _ _ _ _ _ _ _ _ HwellBinds Hclose IHb IHe Ψ HEqΓ
     rw [HEqΓ] at IHe
     rw [HEqΓ] at Hclose
     rw [shiftl_open₀_comm] at IHe
@@ -570,7 +580,7 @@ theorem weakening_strengthened :
     rw [List.length_append, List.length_append, Nat.add_right_comm]
     apply shiftl_closed_at; rw [← List.length_append]; apply Hclose; simp
   case let𝕔 =>
-    intros _ _ _ _ _ _ _ _ HwellBinds Hclose IHb IHe Ψ HEqΓ
+    intros _ _ _ _ _ _ _ _ _ HwellBinds Hclose IHb IHe Ψ HEqΓ
     rw [HEqΓ] at IHe
     rw [HEqΓ] at Hclose
     rw [shiftl_open₀_comm] at IHe
@@ -582,75 +592,75 @@ theorem weakening_strengthened :
     rw [List.length_append, List.length_append, Nat.add_right_comm]
     apply shiftl_closed_at; rw [← List.length_append]; apply Hclose; simp
   case run =>
-    intros _ _ _ _ _ Hclose IH Ψ HEqΓ
+    intros _ _ _ _ _ _ Hclose IH Ψ HEqΓ
     apply typing.run
     apply IH; apply HEqΓ
     rw [shiftl_id]; apply Hclose
     apply closed_inc; apply Hclose; omega
   case pure =>
-    intros _ _ _ _ IH Ψ HEqΓ
+    intros _ _ _ _ _ IH Ψ HEqΓ
     apply typing_reification.pure
     apply IH; apply HEqΓ
   case reify =>
-    intros _ _ _ _ _ IH Ψ HEqΓ
+    intros _ _ _ _ _ _ IH Ψ HEqΓ
     apply typing_reification.reify
     apply IH; apply HEqΓ
   apply Hτ
 
-theorem weakening : ∀ Γ Δ 𝕊 e τ φ, typing Γ 𝕊 e τ φ → typing (Δ ++ Γ) 𝕊 e τ φ :=
+theorem weakening : ∀ Γ Δ σ 𝕊 e τ φ, typing Γ σ 𝕊 e τ φ → typing (Δ ++ Γ) σ 𝕊 e τ φ :=
   by
-  intros Γ Δ 𝕊 e τ φ Hτ
+  intros Γ Δ σ 𝕊 e τ φ Hτ
   rw [← List.nil_append Δ]
   rw [← shiftl_id _ e]
   apply weakening_strengthened
   apply Hτ; rfl
   apply typing_closed; apply Hτ
 
-theorem weakening1 : ∀ Γ 𝕊 e τ𝕒 τ𝕓 φ, typing Γ 𝕊 e τ𝕓 φ -> typing (τ𝕒 :: Γ) 𝕊 e τ𝕓 φ :=
+theorem weakening1 : ∀ Γ σ 𝕊 e τ𝕒 τ𝕓 φ, typing Γ σ 𝕊 e τ𝕓 φ -> typing (τ𝕒 :: Γ) σ 𝕊 e τ𝕓 φ :=
   by
-  intros Γ 𝕊 e τ𝕒 τ𝕓 φ
+  intros Γ σ 𝕊 e τ𝕒 τ𝕓 φ
   rw [← List.singleton_append]
   apply weakening
 
 theorem typing_escape_strengthened :
-  ∀ Γ e τ,
-    typing Γ .dyn e τ ∅ →
-    typing (escape Γ) .stat e τ ∅ :=
+  ∀ Γ σ e τ,
+    typing Γ σ .dyn e τ ∅ →
+    typing (escape Γ) σ .stat e τ ∅ :=
   by
   generalize HEq𝕊 : (.dyn : Stage) = 𝕊
-  intros Γ e τ Hτ
+  intros Γ σ e τ Hτ
   apply
     @typing.rec
-      (fun Γ 𝕊 e τ φ (H : typing Γ 𝕊 e τ φ) =>
+      (fun Γ σ 𝕊 e τ φ (H : typing Γ σ 𝕊 e τ φ) =>
           .dyn = 𝕊 →
-          typing (escape Γ) .stat e τ φ)
-      (fun Γ e τ φ (H : typing_reification Γ e τ φ) => true)
+          typing (escape Γ) σ .stat e τ φ)
+      (fun Γ σ e τ φ (H : typing_reification Γ σ e τ φ) => true)
   <;> (try intros; contradiction)
   case fvar =>
-    intros _ _ x _ Hbinds HwellBinds HEq𝕊
+    intros _ _ _ x _ Hbinds HwellBinds HEq𝕊
     apply typing.fvar
     apply binds_escape; apply Hbinds
     apply well_binding_time_escape; apply HwellBinds
   case lam₁ =>
-    intros _ _ _ _ _ _ _ HwellBinds Hclose IH HEq𝕊
+    intros _ _ _ _ _ _ _ _ HwellBinds Hclose IH HEq𝕊
     rw [← HEq𝕊, escape] at IH
     apply typing.lam₁; rw [← length_escape]
     apply IH; rfl
     apply well_binding_time_escape; apply HwellBinds
     rw [← length_escape]; apply Hclose
   case app₁ =>
-    intros _ _ _ _ _ _ _ _ _ _ _ IHf IHarg HEq𝕊
+    intros _ _ _ _ _ _ _ _ _ _ _ _ IHf IHarg HEq𝕊
     apply typing.app₁
     apply IHf; apply HEq𝕊
     apply IHarg; apply HEq𝕊
   case plus₁ =>
-    intros _ _ _ _ _ _ _ _ IHl IHr HEq𝕊
+    intros _ _ _ _ _ _ _ _ _ IHl IHr HEq𝕊
     apply typing.plus₁
     apply IHl; apply HEq𝕊
     apply IHr; apply HEq𝕊
   case lit₁ => intros; apply typing.lit₁
   case lets =>
-    intros _ _ _ _ _ _ _ _ _ _ HwellBinds Hclose IHb IHe HEq𝕊
+    intros _ _ _ _ _ _ _ _ _ _ _ HwellBinds Hclose IHb IHe HEq𝕊
     rw [← HEq𝕊, escape] at IHe
     apply typing.lets
     apply IHb; apply HEq𝕊
@@ -662,12 +672,12 @@ theorem typing_escape_strengthened :
   apply Hτ; apply HEq𝕊
 
 theorem typing_escape :
-  ∀ Γ e τ,
+  ∀ Γ σ e τ,
     closed_at e 0 →
-    typing Γ .dyn e τ ∅ →
-    typing Γ .stat e τ ∅ :=
+    typing Γ σ .dyn e τ ∅ →
+    typing Γ σ .stat e τ ∅ :=
   by
-  intros Γ e τ Hclose Hτ
+  intros Γ σ e τ Hclose Hτ
   rw [← List.append_nil Γ]; apply weakening
   rw [nil_escape]; apply typing_escape_strengthened
   induction Γ with
